Did a test on function expansion to make sure it's correct.

smtlink/z3_files/smtlink_0S0Y2.py
@@ -1,0 +1,9 @@
+from sys import path
+path.insert(0,"/ubc/cs/home/y/yanpeng/project/ACL2/smtlink/z3_interface")
+from ACL22SMT import to_smt, Q
+s = to_smt()
+var1=s.isReal("var1")
+N=s.isReal("N")
+hypothesis=s.notx(s.lt(2,N))
+conclusion=s.lt((lambda var0:s.ifx(s.ifx(s.notx(s.lt(0,var0)),s.notx(s.lt(0,var0)),s.notx(s.integerp(var0))),1,s.times(var0,var1)))(N),10)
+s.prove(hypothesis, conclusion)
