smtlink/z3_files/smtlink_rilgT.py
@@ -1,0 +1,9 @@
+from sys import path
+path.insert(0,"/ubc/cs/home/y/yanpeng/project/ACL2/smtlink/z3_interface")
+from ACL22SMT import to_smt, Q
+s = to_smt()
+A=s.isReal("A")
+B=s.isReal("B")
+hypothesis=True
+conclusion=s.lt(s.times(2,s.times(A,B)),s.plus(s.times(A,A),s.times(B,B)))
+s.prove(hypothesis, conclusion)
