smtlink/SMT-interpreter.lisp
@@ -5,15 +5,32 @@
 (include-book "config")
 (defttag :tshell)
 
+;; ;; parse-counter-example
+;; (defun parse-counter-example (ce-str)
+;;   "parse-counter-example: parse a counter example string returned by Z3"
+;;   ())
+
+;; ;; fire-session
+;; (defun fire-session (lines)
+;;   ()
+;;   )
+
 ;; SMT-interpreter
+;; If failed, one needs to fire off a raw lisp session
+;; and bind all variables with values.
+;; Need to tell user informations on how to leave the
+;; session.
 (defun SMT-interpreter (filename smt-cnf)
   "SMT-intepreter: get the result returned from calling SMT procedure"
   (mv-let (finishedp exit-status lines)
           (SMT-run filename smt-cnf)
-	  (cond ((equal finishedp nil) 
+	  (cond ((equal finishedp nil)
 		 (cw "Warning: the command was interrupted."))
-		((not (equal exit-status 0)) 
+		((not (equal exit-status 0))
 		 (cw "Z3 failure: ~q0" lines))
 		(t (if (equal (car lines) "proved")
 		       t
-		     (cw "~q0" lines))))))
+         ;;(fire-session lines)
+         (cw "~q0" lines)
+         ))))
+  )
